test_digraph.dfy
@@ -1,0 +1,35 @@
+include "digraph.dfy"
+
+module TestDigraph {
+
+    import DG
+
+    function BuildDigraph(): (r: DG.Digraph)
+        ensures DG.DigraphValid(r)
+    {
+        var g := DG.EmptyDigraph();
+        var node_0 := 0;
+        var node_1 := 1;
+        var node_2 := 2;
+        var node_3 := 3;
+        var node_4 := 4;
+        var g := DG.AddNodeV(g, node_0);
+        var g := DG.AddNodeV(g, node_1);
+        //DG.ConnectNodesPathExists(g, node_0, node_1);
+        var g := DG.ConnectNodesV(g, node_0, node_1);
+        reveal DG.PathValid();
+        assert DG.PathExistsR(g, node_0, node_1);
+        var g := DG.AddNodeV(g, node_2);
+        DG.ConnectNodesPathExists(g, node_1, node_2);
+        var g := DG.ConnectNodesV(g, node_1, node_2);
+        assert DG.PathExistsR(g, node_0, node_1);
+        assert DG.PathExistsR(g, node_1, node_2);
+        assert !DG.PathExistsR(g, node_2, node_1);
+        assert !DG.PathExistsR(g, node_2, node_0);
+        assert DG.PathExistsR(g, node_0, node_2);
+        // 0->1->2
+        // Check that there is a path from 0 to 2.
+        g
+    }
+
+}
